Partial experiments with generation of term-manipulation functions.

src/main/isabelle/Test.thy
@@ -1,13 +1,673 @@
 theory Test
   imports 
- CryptHOL.Cyclic_Group QRHL.QRHL "HOL-Eisbach.Eisbach_Tools" 
-    QRHL.QRHL_Core  Multi_Transfer
+ (* CryptHOL.Cyclic_Group QRHL.QRHL "HOL-Eisbach.Eisbach_Tools"  *)
+QRHL.QRHL
+     (* QRHL.QRHL_Core  Multi_Transfer  *)
+(* QRHL.Prog_Variables *)
 (*   keywords
     "relift_definition" :: thy_goal
  *)
 begin
 
-value "0 = (1::bit)"
+text nothing
+
+no_notation "Order.bottom" ("\<bottom>\<index>")
+no_notation "Order.top" ("\<top>\<index>")
+no_notation "Lattice.meet" (infixl "\<sqinter>\<index>" 70)
+no_notation "Lattice.join" (infixl "\<squnion>\<index>" 65)
+hide_const (open) Order.bottom Order.top
+
+term Order.bottom
+term \<bottom>
+term "a \<sqinter> b"
+term Lattice.meet
+
+definition "assert_equals a b = (a=b)"
+lemma assert_equals_refl: "assert_equals a a" unfolding assert_equals_def by simp
+definition [simp]: "assert_string_neq (a::string) b = (a \<noteq> b)"
+lemma NO_MATCH_I: "NO_MATCH x y" by simp
+
+ML_file "cert_codegen.ML"
+
+(* variables classical xxx :: int begin *)
+
+(* lemma [simp]: "variable_name var_xxx = ''x''" sorry
+lemma [simp]: "variable_name var_xxx = ''x''" *)
+
+(* lemma "variable_name var_xxx = undefined" apply simp oops *)
+
+ML \<open>open Cert_Codegen\<close>
+
+ML \<open>
+fun get_variable_name ctxt v = let
+  val ct = Const(\<^const_name>\<open>variable_name\<close>, fastype_of v --> HOLogic.stringT) $ v |> Thm.cterm_of ctxt
+  val thm = Raw_Simplifier.rewrite_cterm (false,false,false) (K (K NONE)) ctxt ct
+  val rhs = Thm.rhs_of thm |> Thm.term_of
+  val _ = HOLogic.dest_string rhs         
+  in
+    (rhs, fn () => thm RS @{thm meta_eq_to_obj_eq})
+  end
+val get_variable_name_spec : specf = {name="get_variable_name", inputs=["v"], outputs=["n"],
+                                      pattern=\<^prop>\<open>variable_name v = n\<close> |> free_to_var}
+;;
+(* get_variable_name \<^context> @{term var_xxx} *)
+\<close>
+
+ML \<open>
+@{ml_term "string_concat_func a b c"}
+\<close>
+
+ML \<open>
+fun check_func (t,cert) = let
+  val thm = cert ()
+  (* val _ = if Thm.term_of (Thm.rhs_of thm) <> t then raise TERM("check_func",[Thm.prop_of thm, t]) else () *)
+  in (Thm.global_cterm_of (Thm.theory_of_thm thm) t, thm) end
+\<close>
+
+
+(* definition string_concat_func[simp]: "string_concat_func a b c = (a@b = c)" *)
+ML \<open> 
+;;
+string_concat_func \<^context> \<^term>\<open>''hello''\<close> \<^term>\<open>''there''\<close> |> check_func 
+;;
+fun get_variable_name_spec ctxt v = let
+  val ct = Thm.cterm_of ctxt v
+  val thm = Raw_Simplifier.rewrite_cterm (false,false,false) (K (K NONE)) ctxt ct
+  val rhs = Thm.rhs_of thm |> Thm.term_of
+  val _ = HOLogic.dest_string rhs
+  in
+    (rhs, fn () => thm)
+  end
+;;
+val get_variable_name_spec : specf = {name="get_variable_name", inputs=["v"], outputs=["n"],
+                                      pattern=\<^prop>\<open>variable_name v = n\<close> |> free_to_var}
+;;
+(* get_variable_name \<^context> @{term var_xxx} |> check_func *)
+\<close>
+
+
+ML \<open>
+;;
+assert_equals_func \<^context> @{term 123} @{term 123} |> snd |> (fn c => c())
+\<close>
+
+
+lemma index_var1_aux:
+  assumes "variable_name v = vname"
+  assumes "variable_name v1 = v1name"
+  assumes "vname @ ''1'' = v1name'"
+  assumes "assert_equals v1name v1name'"
+  shows "index_var True v = v1"
+  using assms unfolding assert_equals_def using index_var1I by smt
+
+lemma index_var2_aux:
+  assumes "variable_name v = vname"
+  assumes "variable_name v2 = v2name"
+  assumes "vname @ ''2'' = v2name'"
+  assumes "assert_equals v2name v2name'"
+  shows "index_var False v = v2"
+  using assms unfolding assert_equals_def using index_var2I by smt
+
+
+ML \<open>
+fun index_var_func ctxt left (v as Free(n,T)) = let
+  val left' = if left = \<^const>\<open>True\<close> then true else if left = \<^const>\<open>False\<close> then false else raise TERM("index_var_func",[left])
+  fun lr x y = if left' then x else y
+  val v1 = Free(n^lr "1" "2",T)
+  val (vname,vname_cert) = get_variable_name ctxt v
+  val (v1name,v1name_cert) = get_variable_name ctxt v1
+  val (v1name',v1name'_cert) = string_concat_func ctxt vname (lr \<^term>\<open>''1''\<close> \<^term>\<open>''2''\<close>)
+  val ((),eq_cert) = assert_equals_func ctxt v1name v1name'
+  fun cert () = (lr @{thm index_var1_aux} @{thm index_var2_aux}) OF [vname_cert(), v1name_cert(), v1name'_cert(), eq_cert()]
+  in (v1,cert) end
+  | index_var_func _ _ v = raise TERM("index_var_func",[v])
+;;
+val index_var_func_spec = {name="index_var_func", inputs=["left","v"], outputs=["v1"], pattern=\<^prop>\<open>index_var left v = v1\<close> |> free_to_var} : specf
+\<close>
+
+variables classical x :: int begin
+ML \<open>
+index_var_func \<^context> @{term False} @{term "var_x"} |> check_func
+\<close>
+end
+
+lemma index_expression_func:
+  assumes "e \<equiv> expression Q E"
+  assumes "index_vars left Q = Q1"
+  assumes "expression Q1 E \<equiv> e'"
+  shows "index_expression left e = e'"
+  using assms index_expression_def by metis
+
+ML \<open>
+val index_expression_func_spec : specfx = {name="index_expression_func", inputs=["left","e"], outputs=["e'"],
+    pattern=Thm.concl_of @{thm index_expression_func}, thms=["index_expression_func"], 
+    fallback="fn (left,e) => raise TERM(\"index_expression_func\",[left,e])"}
+\<close>
+
+
+lemma index_vars_unit_func:
+  assumes "X \<equiv> variable_unit"
+  assumes "variable_unit \<equiv> X'"
+  shows "index_vars left X = X'"
+  using assms index_vars_unit by metis
+
+lemma index_vars_singleton_func:
+  assumes "X \<equiv> variable_singleton x"
+  assumes "index_var left x = x1"
+  assumes "variable_singleton x1 \<equiv> X'"
+  shows "index_vars left X = X'"
+  using assms index_vars_singleton by metis
+
+lemma index_vars_concat_func:
+  assumes "X \<equiv> variable_concat Y Z"
+  assumes "index_vars left Y = Y1"
+  assumes "index_vars left Z = Z1"
+  assumes "variable_concat Y1 Z1 \<equiv> X'"
+  shows "index_vars left X = X'"
+  using assms index_vars_concat by metis
+
+ML \<open>
+val index_vars_func_spec : specfx = {name="index_vars", inputs=["left","X"], outputs=["X'"],
+  thms= ["index_vars_unit_func","index_vars_singleton_func","index_vars_concat_func"],
+  pattern=Thm.concl_of @{thm index_vars_singleton_func}, fallback="fn (left,X) => raise TERM(\"index_vars_concat_func\",[left,X])"}
+\<close>
+
+lemma subst_expression_func_unit:
+  assumes "s == substitute1 x f"
+  assumes "e == expression variable_unit E"
+  assumes "expression variable_unit E == e'"
+  shows "subst_expression s e = e'"
+  using assms Encoding.subst_expression_unit_aux by metis
+
+lemma subst_expression_func_singleton_same:
+  assumes "s == substitute1 x (expression R F)"
+  assumes "e == expression \<lbrakk>x\<rbrakk> E"
+  assumes "expression R (\<lambda>r. E (F r)) == e'"
+  shows "subst_expression s e = e'"
+  using assms Encoding.subst_expression_singleton_same_aux by metis
+
+lemma subst_expression_func_singleton_notsame:
+  assumes "s == substitute1 x f"
+  assumes "e == expression \<lbrakk>y\<rbrakk> E"
+  assumes "variable_name x = xn"
+  assumes "variable_name y = yn"
+  assumes neq: "assert_string_neq xn yn"
+  assumes "e == e'"
+  shows "subst_expression s e = e'"
+  using neq unfolding assms(1,2) assms(3,4,6)[symmetric] assert_string_neq_def
+  using Encoding.subst_expression_singleton_notsame_aux by metis
+
+lemma subst_expression_func_concat_id:
+  assumes "s == substitute1 x f"
+  assumes "e == expression (variable_concat Q1 Q2) (\<lambda>x. x)"
+  assumes "subst_expression (substitute1 x f) (expression Q1 (\<lambda>x. x)) = expression Q1' e1"
+  assumes "subst_expression (substitute1 x f) (expression Q2 (\<lambda>x. x)) = expression Q2' e2"
+  assumes "expression (variable_concat Q1' Q2') (\<lambda>(x1,x2). (e1 x1, e2 x2)) == e'"
+  shows "subst_expression s e = e'"
+  using assms Encoding.subst_expression_concat_id_aux by metis
+
+lemma subst_expression_func_id_comp:
+  assumes "s == substitute1 x f"
+  assumes "e == expression Q E"
+  assumes "NO_MATCH (\<lambda>x::unit. x) E"
+  assumes "subst_expression (substitute1 x f) (expression Q (\<lambda>x. x)) = expression Q' g"
+  assumes "expression Q' (\<lambda>x. E (g x)) == e'"
+  shows "subst_expression s e = e'"
+  using assms(4) unfolding assms(1-2) assms(5)[symmetric]
+  using Encoding.subst_expression_id_comp_aux by metis
+
+ML \<open>
+val subst_expression_func_spec : specfx = {
+  name="subst_expression_func",
+  inputs=["s","e"], outputs=["e'"], pattern= @{thm subst_expression_func_id_comp} |> Thm.concl_of,
+  thms= ["subst_expression_func_unit","subst_expression_func_concat_id",
+               "subst_expression_func_singleton_same","subst_expression_func_singleton_notsame",
+               "subst_expression_func_concat_id", "subst_expression_func_id_comp"],
+  fallback="fn (s,e) => raise TERM(\"subst_expression_func\",[s,e])"}
+\<close>
+
+
+
+lemma wp_skip_func:
+  assumes "c == []" and "d == []" and "B == A"
+  shows "qrhl A c d B"
+  unfolding assms by (rule wp_skip)
+
+lemma wp1_assign_func:
+  fixes x e c d A B
+  assumes "c == [assign x e]" and "d == []"
+  assumes "index_var True x = x1"
+  assumes "index_expression True e = e1"
+  assumes "subst_expression (substitute1 x1 e1) B = A"
+  shows "qrhl A c d B"
+  using assms wp1_assign by metis
+
+lemma wp2_assign_func:
+  fixes x e c d A B
+  assumes "d == [assign x e]" and "c == []"
+  assumes "index_var False x = x1"
+  assumes "index_expression False e = e1"
+  assumes "subst_expression (substitute1 x1 e1) B = A"
+  shows "qrhl A c d B"
+  using assms wp2_assign by metis
+
+lemma wp1_sample_func:
+  fixes A B c d x e
+  assumes "d == []" and "c == [sample x e]" 
+  assumes "index_var True x = x1"
+  assumes "index_expression True e = e1"
+(* TODO: all-quants probably don't work! *)
+  assumes "\<And>z. subst_expression (substitute1 x1 (const_expression z)) B = B' z"
+(* TODO: implement map_expression2 *)
+  assumes "map_expression2' (\<lambda>e' B'. Cla[weight e' = 1] \<sqinter> (INF z:supp e'. B' z)) e1 B' == A"
+  shows "qrhl A c d B"
+  unfolding assms(1-2) assms(3-6)[symmetric] by (rule wp1_sample)
+
+lemma wp2_sample_func:
+(*TODO*)
+  fixes A B c d x e
+  assumes "c == []" and "d == [sample x e]" 
+  defines "e' \<equiv> index_expression False e"
+  defines "B' z \<equiv> subst_expression (substitute1 (index_var False x) (const_expression z)) B"
+  assumes "map_expression2' (\<lambda>e' B'. Cla[weight e' = 1] \<sqinter> (INF z:supp e'. B' z)) e' B' == A"
+  shows "qrhl A c d B"
+  unfolding assms(1-4) assms(5)[symmetric] by (rule wp2_sample)
+
+lemma wp1_qapply_func:
+(*TODO*)
+  fixes A B Q e
+  assumes "d == []" and "c == [qapply Q e]"
+  defines "Q\<^sub>1 \<equiv> index_vars True Q"
+  assumes "map_expression2 (\<lambda>e\<^sub>1 B. Cla[isometry e\<^sub>1] \<sqinter> (adjoint (e\<^sub>1\<guillemotright>Q\<^sub>1) \<cdot> (B \<sqinter> (e\<^sub>1\<guillemotright>Q\<^sub>1 \<cdot> top)))) (index_expression True e) B \<equiv> A"
+  shows "qrhl A c d B"
+  unfolding assms(1-3) assms(4)[symmetric] by (rule wp1_qapply)
+
+lemma wp2_qapply_func:
+(*TODO*)
+  fixes A B Q e
+  assumes "c == []" and "d == [qapply Q e]"
+  defines "Q\<^sub>1 \<equiv> index_vars False Q"
+  assumes "map_expression2 (\<lambda>e\<^sub>1 B. Cla[isometry e\<^sub>1] \<sqinter> (adjoint (e\<^sub>1\<guillemotright>Q\<^sub>1) \<cdot> (B \<sqinter> (e\<^sub>1\<guillemotright>Q\<^sub>1 \<cdot> top)))) (index_expression False e) B \<equiv> A"
+  shows "qrhl A c d B"
+  unfolding assms(1-3) assms(4)[symmetric] by (rule wp2_qapply)
+
+lemma wp1_measure_func:
+(*TODO*)
+  fixes A B x Q e
+  assumes "d == []" and "c == [measurement x Q e]"
+  defines "e\<^sub>1 \<equiv> index_expression True e"
+  defines "B' z \<equiv> subst_expression (substitute1 (index_var True x) (const_expression z)) B"
+  defines "\<And>e\<^sub>1 z. ebar e\<^sub>1 z \<equiv> ((mproj e\<^sub>1 z)\<guillemotright>(index_vars True Q)) \<cdot> top"
+  assumes "map_expression2' (\<lambda>e\<^sub>1 B'. Cla[mtotal e\<^sub>1] \<sqinter> 
+           (INF z. ((B' z \<sqinter> ebar e\<^sub>1 z) + ortho (ebar e\<^sub>1 z)))) e\<^sub>1 B' == A"
+  shows "qrhl A c d B"
+  unfolding assms(1-5) assms(6)[symmetric] by (rule wp1_measure)
+
+lemma wp2_measure_func:
+(*TODO*)
+  fixes A B x Q e
+  assumes "c == []" and "d == [measurement x Q e]"
+  defines "e\<^sub>1 \<equiv> index_expression False e"
+  defines "B' z \<equiv> subst_expression (substitute1 (index_var False x) (const_expression z)) B"
+  defines "\<And>e\<^sub>1 z. ebar e\<^sub>1 z \<equiv> ((mproj e\<^sub>1 z)\<guillemotright>(index_vars False Q)) \<cdot> top"
+  assumes "map_expression2' (\<lambda>e\<^sub>1 B'. Cla[mtotal e\<^sub>1] \<sqinter> 
+           (INF z. ((B' z \<sqinter> ebar e\<^sub>1 z) + ortho (ebar e\<^sub>1 z)))) e\<^sub>1 B' == A"
+  shows "qrhl A c d B"
+  unfolding assms(1-5) assms(6)[symmetric] by (rule wp2_measure)
+
+lemma wp1_qinit_func:
+(*TODO*)
+  fixes A B e Q
+  assumes "d==[]" and "c == [qinit Q e]"
+  assumes "map_expression2 (\<lambda>e\<^sub>1 B. Cla[norm e\<^sub>1 = 1] \<sqinter> (B \<div> e\<^sub>1 \<guillemotright> (index_vars True Q)))
+           (index_expression True e) B == A"
+  shows "qrhl A c d B"
+  unfolding assms(1-2) assms(3)[symmetric] by (rule wp1_qinit)
+
+lemma wp2_qinit_func:
+(*TODO*)
+  fixes A B e Q
+  assumes "c == []" and "d == [qinit Q e]"
+  assumes "map_expression2 (\<lambda>e\<^sub>1 B. Cla[norm e\<^sub>1 = 1] \<sqinter> (B \<div> e\<^sub>1 \<guillemotright> (index_vars False Q)))
+           (index_expression False e) B == A"
+  shows "qrhl A c d B"
+  unfolding assms(1-2) assms(3)[symmetric] by (rule wp2_qinit)
+
+lemma wp1_if_func:
+(*TODO*)
+  fixes e p1 p2 B
+  assumes "d == []" and "c == [ifthenelse e p1 p2]"
+  assumes "qrhl wp_true p1 [] B"
+  assumes "qrhl wp_false p2 [] B"
+  assumes "map_expression3 (\<lambda>e\<^sub>1 wp_true wp_false. (Cla[\<not>e\<^sub>1] + wp_true) \<sqinter> (Cla[e\<^sub>1] + wp_false))
+           (index_expression True e) wp_true wp_false == A"
+  shows "qrhl A c d B"
+  unfolding assms(1-2) assms(5)[symmetric] using assms(3,4) by (rule wp1_if)
+
+lemma wp2_if_func:
+(*TODO*)
+  fixes e p1 p2 B
+  assumes "c == []" and "d == [ifthenelse e p1 p2]"
+  assumes "qrhl wp_true [] p1 B"
+  assumes "qrhl wp_false [] p2 B"
+  assumes "map_expression3 (\<lambda>e\<^sub>1 wp_true wp_false. (Cla[\<not>e\<^sub>1] + wp_true) \<sqinter> (Cla[e\<^sub>1] + wp_false))
+           (index_expression False e) wp_true wp_false == A"
+  shows "qrhl A c d B"
+  unfolding assms(1-2) assms(5)[symmetric] using assms(3,4) by (rule wp2_if)
+
+lemma wp1_block_func:
+(*TODO*)
+  assumes "d == []" and "c == [block p]"
+  assumes "qrhl A p [] B"
+  shows "qrhl A c d B"
+  unfolding assms(1,2) using assms(3) by (rule wp1_block)
+
+lemma wp2_block_func:
+(*TODO*)
+  assumes "c == []" and "d == [block p]"
+  assumes "qrhl A [] p B"
+  shows "qrhl A c d B"
+  unfolding assms(1,2) using assms(3) by (rule wp2_block)
+
+lemma wp1_cons_func:
+  assumes "d == []" and "c == p#ps"
+  assumes "NO_MATCH ([]::unit list) ps"
+  assumes "qrhl B' ps [] B" and "qrhl A [p] [] B'"
+  shows "qrhl A c d B"
+  unfolding assms(1,2) using assms(4,5) by (rule wp1_cons[rotated])
+
+lemma wp2_cons_func:
+  assumes "c == []" and "d == p#ps"
+  assumes "NO_MATCH ([]::unit list) ps"
+  assumes "qrhl B' [] ps B"
+    and "qrhl A [] [p] B'"
+  shows "qrhl A c d B"
+  unfolding assms(1,2) using assms(4,5) by (rule wp2_cons[rotated])
+
+
+
+
+(* lemmas wp_func = wp_skip_func wp1_assign_func wp2_assign_func (* wp1_sample_func TODO *) wp2_sample_func
+  wp1_qapply_func wp2_qapply_func wp1_measure_func wp2_measure_func wp1_if_func wp2_if_func
+  wp1_block_func wp2_block_func wp1_cons_func wp2_cons_func *)
+
+
+
+
+(* ML \<open>
+val thm_by_id = Synchronized.var "thm_by_id" Inttab.empty : thm Inttab.table Synchronized.var
+fun store_thm thm = let val id = serial () 
+                        val _ = Synchronized.change thm_by_id (Inttab.update_new (id,thm))
+                    in id end
+fun get_thm_by_id id = Inttab.lookup (Synchronized.value thm_by_id) id |> the
+\<close>
+ *)
+
+(* ML \<open>
+structure Data = Theory_Data (
+  type T = thm Inttab.table
+  (* fun init _ = Inttab.empty *)
+  val empty = Inttab.empty
+  fun merge _ = Inttab.empty
+  val extend = I
+)
+fun get_thm ctxt id = Inttab.lookup (Data.get ctxt) id |> the
+fun thm_antiq (conf:conf) thm =
+  let val id = serial ()
+      val ctxt = Data.map (Inttab.update_new (id,thm)) (!(#ctxt conf))
+      val (var,ctxt) = ML_Context.variant "thm" ctxt
+      val prepare = "val " ^ var ^ " = get_thm \<^context> " ^ ML_Syntax.print_int id
+      val retrieve = (* ML_Context.struct_name ctxt ^ "." ^ *) var
+      val _ = #ctxt conf := ctxt
+  in
+    (prepare,retrieve)
+  end
+\<close> *)
+
+
+ML \<open>
+fun specf_to_specfx ({name,inputs,outputs,pattern} : specf) = {name=name,fallback="",inputs=inputs,outputs=outputs,pattern=pattern,thms=[]} : specfx
+\<close>
+
+
+ML \<open>
+val spec_wp = 
+{name="wp", thms= 
+["wp_skip_func","wp1_assign_func","wp2_assign_func", (* "wp1_sample_func", *) "wp2_sample_func",
+  "wp1_qapply_func", "wp2_qapply_func", "wp1_measure_func", "wp2_measure_func", "wp1_if_func", "wp2_if_func",
+  "wp1_block_func", "wp2_block_func", "wp1_cons_func", "wp2_cons_func"],
+inputs=["c","d","B"], outputs=["A"], fallback="fn (c,d,B) => raise TERM(\"wp\",[c,d,B])", pattern=Thm.concl_of @{thm wp_skip_func}} : specfx
+val spec = [
+  spec_wp,
+  specf_to_specfx index_var_func_spec,
+  specf_to_specfx get_variable_name_spec,
+  specf_to_specfx assert_string_neq_func_spec,
+  specf_to_specfx NO_MATCH_func_spec,
+  index_expression_func_spec,
+  index_vars_func_spec,
+  subst_expression_func_spec
+]
+\<close>
+
+
+
+ML \<open>
+;;
+print_comment "This (* is *) cool (******)"
+\<close>
+
+
+
+
+
+
+ML \<open>
+(* TODO make work *)
+thm_to_fun \<^context> (empty_conf (hd spec)) spec "wp1_sample_func" "f" ["c","d","B"] ["A"] |> writeln
+\<close>
+
+
+ML \<open>
+;;
+val _ = thms_to_fun \<^context> spec spec_wp |> tracing
+\<close>
+
+ML \<open>
+\<close>
+
+
+
+ML \<open>
+(* val path = Path.append (Resources.master_directory \<^theory>) (Path.make ["test.ML"]) *)
+val code = thms_to_funs \<^context> spec "Test" "test.ML"
+(* val code = "val x = 1;;" *)
+(* val written = File.write path code *)
+(* val _ = ML_Context.eval_file ML_Compiler.flags path *)
+(* val pos = Path.position path *)
+(* val lex = ML_Lex.read_pos pos code *)
+(* val res = ML_Context.eval_in (SOME ctxt) ML_Compiler.flags pos lex *)
+(* val res = ML_Context.eval_file ML_Compiler.flags path *)
+\<close>
+
+ML_file "test.ML"
+
+(* declare[[show_brackets]] *)
+(* print_attributes *)
+
+declare[[show_abbrevs=false,eta_contract=false]]
+ML \<open>
+\<^term>\<open>(%x::bool. x)\<close> $ \<^term>\<open>True\<close> |> Thm.cterm_of \<^context> 
+\<close>
+
+term "(%x. x) x"
+term "(%x. f x)"
+
+ML \<open>
+fun rewrite_thm_as thm ct = let
+val eq = Thm.transitive (Thm.beta_conversion true (Thm.cprop_of thm)) (Thm.beta_conversion true ct |> Thm.symmetric)
+val thm' = Thm.equal_elim eq thm
+in thm' end
+\<close>
+
+ML \<open>
+local
+val ctxt = \<^context>
+val assm = @{prop "\<And>z. subst_expression (substitute1 x1 (const_expression z)) B = B' z"} |> free_to_var
+val termvars = Symtab.make(map(fn n=>(n,n))["B","t_b","t_a","x1","z"])
+val conf = (empty_conf (hd spec))
+
+val _ = assm |> Thm.cterm_of ctxt
+val ((z,T),assm') = Logic.dest_all assm
+(* val _ = (z,T) |> @{print} *)
+val _ = assm' |> Thm.cterm_of ctxt
+val vars = Term.add_vars assm [] |> map (fst o fst)
+val outputs = vars |> filter (not o Symtab.defined termvars)
+val outputs_z = Name.variant_list vars (outputs |> map (fn n => n ^ "_" ^ z))
+val subst = outputs ~~ outputs_z |> Symtab.make
+fun s (t as Var((n,0),T') $ Free z') =
+    (case (Symtab.lookup subst n, z'=(z,T)) of
+      (SOME nz, true) => Var((nz,0),T' |> dest_funT |> snd)
+    | _ => t)
+  | s (t1 $ t2) = s t1 $ s t2
+  | s (Abs(n,T,t)) = Abs(n,T,s t)
+  | s t = t
+val assm'' = s assm'
+val _ = assm'' |> Thm.cterm_of ctxt
+
+val ((code,cert'),(termvars,ctxt)) = code_for_assumption ctxt termvars conf spec assm''
+val code = "local" :: map indent' code
+(* val _ = @{print} termvars *)
+(* val _ = @{print} termvars *)
+(* val _ = @{print} cert' *)
+
+val comment = print_comment "TODO: comment"
+fun abscode1 (v,vz) (ctxt,termvars,checks) = let 
+  val (v',(ctxt,termvars,checks)) = print_var_pattern v (ctxt,termvars,checks)
+  val T' = print_typ termvars T
+  val vz' = print_var termvars vz
+  in ("val "^v'^" = absfree ("^ML_Syntax.print_string z^","^T'^") "^vz', (* SHouldn't z be quoted in some way? TODO *)
+      (ctxt,termvars,checks)) end
+val (abscode,(ctxt,termvars,checks)) = fold_map abscode1 (Symtab.dest subst) (ctxt,termvars,[])
+val _ = if null checks then () else error "checks not empty"
+val (certvar,ctxt) = ML_Context.variant "cert" ctxt
+val certcode = "fun "^certvar^" () = generalize_thm_to ctxt " ^ ML_Syntax.atomic cert' ^ " " ^ ML_Syntax.atomic (print_term termvars assm)
+  ^ " TODO: (" ^ "\"z\",t_a)"
+val code = code @ ["in", comment] @ abscode @ [certcode,"end"]
+
+val termvars = fold Symtab.delete outputs_z termvars
+
+val _ = code |> String.concatWith "\n" |> tracing
+
+(* Generate: cert *)
+
+in end
+\<close>
+
+ML \<open>
+fun generalize_thm_to ctxt thm prop (v,T) = let
+  val thm' = thm |> Thm.generalize ([],["v"]) 0 |> Thm.forall_intr (Thm.cterm_of ctxt (Free(v,T)))
+  val thm'' = rewrite_thm_as thm' (Thm.cterm_of ctxt prop)
+  in thm'' end
+\<close>
+
+
+
+variables classical x :: nat begin
+ML \<open>
+local
+val ctxt = \<^context>
+val t_a = @{typ "nat"}
+val t_b = @{typ "nat"}
+val x1 = @{term "var_x1"}
+val B = @{term "Expr[Suc x1]"}
+open Test
+in
+
+local
+  (* Assumption: subst_expression (substitute1 ?x1.0 (expression variable_unit (\<lambda>_. z))) ?B = ?B'_z
+     Handled using function subst_expression_func *)
+  val (((b_z)), cert)
+           = subst_expression_func ctxt (Term.$ (Term.$ (Term.Const ("Expressions.substitute1", Term.Type ("fun", [Term.Type ("Prog_Variables.variable", [t_a]), Term.Type ("fun", [Term.Type ("Expressions.expression", [t_a]), Term.Type ("Expressions.substitution", [])])])), x1), Term.$ (Term.$ (Term.Const ("Expressions.expression", Term.Type ("fun", [Term.Type ("Prog_Variables.variables", [Term.Type ("Product_Type.unit", [])]), Term.Type ("fun", [Term.Type ("fun", [Term.Type ("Product_Type.unit", []), t_a]), Term.Type ("Expressions.expression", [t_a])])])), Term.Const ("Prog_Variables.variable_unit", Term.Type ("Prog_Variables.variables", [Term.Type ("Product_Type.unit", [])]))), Term.Abs ("uu_", Term.Type ("Product_Type.unit", []), Term.Free ("z", t_a))))) (B)
+in
+(* TODO: comment *)
+val b = absfree ("z",t_a) b_z
+fun certa () = generalize_thm_to ctxt (cert ()) (Term.$ (Term.Const ("Pure.all", Term.Type ("fun", [Term.Type ("fun", [t_a, Term.Type ("prop", [])]), Term.Type ("prop", [])])), Term.Abs ("z", t_a, Term.$ (Term.Const ("HOL.Trueprop", Term.Type ("fun", [Term.Type ("HOL.bool", []), Term.Type ("prop", [])])), Term.$ (Term.$ (Term.Const ("HOL.eq", Term.Type ("fun", [Term.Type ("Expressions.expression", [t_b]), Term.Type ("fun", [Term.Type ("Expressions.expression", [t_b]), Term.Type ("HOL.bool", [])])])), Term.$ (Term.$ (Term.Const ("Expressions.subst_expression", Term.Type ("fun", [Term.Type ("Expressions.substitution", []), Term.Type ("fun", [Term.Type ("Expressions.expression", [t_b]), Term.Type ("Expressions.expression", [t_b])])])), Term.$ (Term.$ (Term.Const ("Expressions.substitute1", Term.Type ("fun", [Term.Type ("Prog_Variables.variable", [t_a]), Term.Type ("fun", [Term.Type ("Expressions.expression", [t_a]), Term.Type ("Expressions.substitution", [])])])), x1), Term.$ (Term.$ (Term.Const ("Expressions.expression", Term.Type ("fun", [Term.Type ("Prog_Variables.variables", [Term.Type ("Product_Type.unit", [])]), Term.Type ("fun", [Term.Type ("fun", [Term.Type ("Product_Type.unit", []), t_a]), Term.Type ("Expressions.expression", [t_a])])])), Term.Const ("Prog_Variables.variable_unit", Term.Type ("Prog_Variables.variables", [Term.Type ("Product_Type.unit", [])]))), Term.Abs ("uu_", Term.Type ("Product_Type.unit", []), Term.Bound 1)))), B)), Term.$ (b, Term.Bound 0))))))
+  ("z",t_a)
+end 
+
+
+end
+;;
+b |> Thm.cterm_of \<^context>
+;;
+certa ()
+;;
+certa () 
+|> Thm.prop_of
+(* |> Term.dest_comb |> snd *)
+(* |> (fn (Abs(_,_,body)) => body) *)
+|> Logic.dest_all |> snd
+|> HOLogic.dest_Trueprop
+|> Term.dest_comb |> snd
+ (* |>Thm.cterm_of \<^context> *)
+\<close>
+
+ML \<open>
+val ctxt = \<^context>
+val t_b = @{typ "nat"}
+val x1 = @{term "var_x1"}
+val z = @{term "z::nat"}
+val B = @{term "Expr[Suc x1]"}
+
+(* Assumption: subst_expression (substitute1 ?x1.0 (const_expression ?z)) ?B = ?B'z
+   Handled using function subst_expression_func *)
+
+val (((b_z)), cert)
+         = Test.subst_expression_func ctxt (Term.$ (Term.$ (Term.Const ("Expressions.substitute1", Term.Type ("fun", [Term.Type ("Prog_Variables.variable", [t_b]), Term.Type ("fun", [Term.Type ("Expressions.expression", [t_b]), Term.Type ("Expressions.substitution", [])])])), x1), Term.$ (Term.$ (Term.Const ("Expressions.expression", Term.Type ("fun", [Term.Type ("Prog_Variables.variables", [Term.Type ("Product_Type.unit", [])]), Term.Type ("fun", [Term.Type ("fun", [Term.Type ("Product_Type.unit", []), t_b]), Term.Type ("Expressions.expression", [t_b])])])), Term.Const ("Prog_Variables.variable_unit", Term.Type ("Prog_Variables.variables", [Term.Type ("Product_Type.unit", [])]))), Term.Abs ("uu_", Term.Type ("Product_Type.unit", []), z)))) (B) 
+val B' = absfree ("z",@{typ int}) b_z
+val thm = cert()
+val prop = @{cprop "\<And>z. subst_expression (substitute1 var_x1 (const_expression z)) (expression \<lbrakk>var_x1\<rbrakk> (%x. Suc x)) = (\<lambda>z. const_expression (Suc z)) z"}
+val thm' = thm |> Thm.generalize ([],["z"]) 0 |> Thm.forall_intr (Thm.cterm_of \<^context> (Var(("z",0),@{typ nat})))
+val thm'' = rewrite_thm_as thm' prop
+\<close>
+end
+
+(* ML \<open>
+val _ = Theory.setup (ML_Antiquotation.declaration \<^binding>\<open>lemma_to_fun\<close>
+(Scan.succeed()) (fn _ => fn _ => fn ctxt => (lemma_to_fun ctxt spec |> apfst K)))
+\<close> *)
+
+variables classical x :: bool and classical y :: bool begin
+(* declare [[show_types,show_consts]] *)
+ML \<open>
+Test.index_vars \<^context> @{term True} @{term "\<lbrakk>var_x,var_y\<rbrakk>"} |> check_func
+\<close>
+
+ML \<open>
+Test.wp \<^context> @{term "[assign var_x Expr[undefined]]"} @{term "[] :: program list"} @{term "Expr[top::predicate]"}
+|> check_func
+\<close>
+
+
+ML \<open>
+(* TODO should simplif the nested prod-case's *)
+Test.subst_expression_func \<^context> @{term "substitute1 (var_x1::bool variable) (const_expression True)"}
+@{term "Expr[Cla[x1=x2]]"}
+|> check_func
+\<close>
+end
+
+
+variables classical x :: int begin
+ML \<open>
+wp \<^context> @{term "[assign var_x Expr[x*x], assign var_x Expr[x*x]]"} @{term "[] :: program list"} @{term "Expr[Cla[x1=x2]]"}
+|> check_func
+\<close>
+end
+
+
+
+(* value "0 = (1::bit)"
 
 typedef stuff = "UNIV :: nat set" by simp
 
@@ -50,7 +710,7 @@ lemma "stuff1.all = stuff2.all"
   apply transfer
   by simp
   
-
+ *)
 
 
 ML \<open>
@@ -122,8 +782,8 @@ method_setup cheat = \<open>Scan.lift (Parse.position Parse.text) >> (fn (txt,po
 declare[[smt_oracle=true]]
 
 lemma theo: "1=1"
-  apply (rule trans[of _ 1])
-   apply (cheat 1)
+  (* apply (rule trans[of _ 1]) *)
+   (* apply (cheat 1) *)
   by smt
 
 ML \<open>
